\documentclass{article}
\usepackage[margin=1.25in]{geometry}
\usepackage{amsmath, amsfonts}
\usepackage{enumitem}

\newcommand{\trace}{\mathrm{trace}}
\newcommand{\R}{\mathbb{R}}

\begin{document}
\begin{enumerate}[label=\textbf{5.\arabic*.}]
    \setcounter{enumi}{2}
    
    \item $T_{\alpha+\beta} = T_{\alpha}T_{\beta} = T_{\beta}T_{\alpha}$
    
    \addtocounter{enumi}{2}

    \item Define $T, T':M_{n\times n}^{\R} \rightarrow \R$ with
    $T(X) =  \trace(AX)$ and $T'(X) = \trace(XA)$. 
    Both $T$ and $T'$ are linear transformations
    \begin{align*} T(\alpha_1 X_1 + \alpha_2 X_2) &=
    \trace(\alpha_1 X_1 + \alpha_2 X_2) \\
    &= \trace(\alpha_1 X_1) + \trace(\alpha_2 X_2) \\
    &= \alpha_1\trace(X_1) + \alpha_2\trace(X_2) \\
    &= \alpha_1 T(X_1) + \alpha_2 T(X_2)
    \end{align*}
    Over the standard basis in
    $M_{n\times n}^{\R}$ (a system of $e_{i, j}$ matrices of all entries zero
    but the $(i, j)$th as 1) transformations are
    $T(e_{i, j}) = \sum_k\sum_l a_{lk}(e_{i, j})_{kl} = a_{ji}(e_{i, j})_{ij}$,
    and
    $T'(e_{i, j}) = \sum_k\sum_l (e_{i, j})_{kl}a_{lk} = (e_{i, j})_{ij}a_{ji}$
    It follows  $T = T'$, or $\trace(AX) = \trace(XA)$. And, for $X = B$,
    $\trace(AB) = \trace(BA)$.

    Alternatively, \begin{align*} \trace(AB) &= \sum_{i}\sum_{k}a_{ik}b_{ki} \\
    &= \begin{aligned} &a_{11}b_{11} + \ldots + a_{1n}b_{n1} \\
        &+ a_{21}b_{12} + \ldots + a_{2n}b_{n2} \\
        &\qquad \vdots \\
        &+ a_{n1}b_{1n} + \ldots + a_{nn}b_{nn} \end{aligned} \\
    &= \sum_{k}\sum_{i} b_{ki}a_{ik} \\
    &= \trace(BA)
    \end{align*}
\end{enumerate}
\end{document}